\documentclass[solutions.tex]{subfiles}

\xtitle

\begin{document}
\maketitle
\begin{exercise}
Show that the inner product defined by Eq. $1.2$ satisfies all the
axioms of inner products.
\end{exercise}
\hrr
Let us recall the two axioms in question:
\begin{axiom}\ \\
$$ \bra{C} \Big( \ket{A} + \ket{B} \Big) = \braket{C}{A} + \braket{C}{B} $$
\end{axiom}
\begin{axiom}
$$ \braket{B}{A} = \braket{A}{B}^{*} $$
Where $z^{*}$ is the complex conjugate of $z\in\mathbb{C}$
\end{axiom}

And let us recall Eq. $1.2$ of the book:

\begin{align*}
	\braket{B}{A} &=
		\begin{pmatrix}
			\beta_1^* & \beta_2^* & \beta_3^* & \beta_4^* & \beta_5^* \\
		\end{pmatrix}
		\begin{pmatrix}
			\alpha_1 \\
			\alpha_2 \\
			\alpha_3 \\
			\alpha_4 \\
			\alpha_5 \\
		\end{pmatrix} \\
	~ &= \beta_1^*\alpha_1 + \beta_2^*\alpha_2 + \beta_3^*\alpha_3 +
	\beta_4^*\alpha_4 + \beta_5^*\alpha_5 \\
\end{align*}

For the first axiom, considering $\bra{C} = (\gamma_i^*)$:

\begin{align*}
\bra{C} \Big( \ket{A} + \ket{B} \Big) &=
\begin{pmatrix}
\gamma_1^* & \gamma_2^* & \gamma_3^* & \gamma_4^* & \gamma_5^* \\
\end{pmatrix}
\begin{pmatrix}
\alpha_1 + \beta_1 \\
\alpha_2 + \beta_2 \\
\alpha_3 + \beta_3 \\
\alpha_4 + \beta_4 \\
\alpha_5 + \beta_5 \\
\end{pmatrix}
\\
~ &= \gamma_1^*(\alpha_1+\beta_1) + \gamma_2^*(\alpha_2+\beta_2) +
\gamma_3^*(\alpha_3+\beta_3) + \gamma_4^*(\alpha_4+\beta_4) +
\gamma_5^*(\alpha_5+\beta_5) \\
~ &= \big(\gamma_1^*\alpha_1 + \gamma_2^*\alpha_2 + \gamma_3^*\alpha_3 +
\gamma_4^*\alpha_4 + \gamma_5^*\alpha_5 \big) +
\big(\gamma_1^*\beta_1 + \gamma_2^*\beta_2 + \gamma_3^*\beta_3 +
\gamma_4^*\beta_4 + \gamma_5^*\beta_5 \big) \\
~ &=
\begin{pmatrix}
	\gamma_1^* & \gamma_2^* & \gamma_3^* & \gamma_4^* & \gamma_5^* \\
\end{pmatrix}
\begin{pmatrix}
	\alpha_1 \\
	\alpha_2 \\
	\alpha_3 \\
	\alpha_4 \\
	\alpha_5 \\
\end{pmatrix} +
\begin{pmatrix}
	\gamma_1^* & \gamma_2^* & \gamma_3^* & \gamma_4^* & \gamma_5^* \\
\end{pmatrix}
\begin{pmatrix}
	\beta_1 \\
	\beta_2 \\
	\beta_3 \\
	\beta_4 \\
	\beta_5 \\
\end{pmatrix} \\
~ &= \braket{C}{A} + \braket{C}{B} \qed
\end{align*}

Before diving into the second axiom, let us observe that for
$(a, b) = (x_a+iy_a, x_b+iy_b) \in\mathbb{C}^2$:
\begin{align*}
	(ab)^* &= \Big((x_a+iy_a)\times(x_b+iy_b)\Big)^* \\
	~ &= \Big(x_ax_b - y_ay_b +i(x_by_a +x_ay_b)\Big)^* \\
	~ &= x_ax_b - y_ay_b -i(x_by_a +x_ay_b) \\
	~ &= (x_a-iy_a)\times(x_b-iy_b) \\
	~ &= a^*b^* \\
\end{align*}

Or, perhaps more simply using complex numbers' exponential's form:
\begin{align*}
	(ab)^* &= \Big(r_ar_be^{i(\theta_a+\theta_b)}\Big)^* \\
	~ &= r_ar_be^{-i(\theta_a+\theta_b)} \\
	~ &= a^*b^* \\
\end{align*}

Hence, regarding the second axiom:

\begin{align*}
	\braket{B}{A} &= \Big(\big(\braket{B}{A}\big)^*\Big)^* \\
	~ &= \Big(\big(\beta_1^*\alpha_1 + \beta_2^*\alpha_2 + \beta_3^*\alpha_3 +
	\beta_4^*\alpha_4 + \beta_5^*\alpha_5\big)^*\Big)^* \\
	~ &= \Big(\beta_1\alpha_1^* + \beta_2\alpha_2^* + \beta_3\alpha_3^* +
	\beta_4\alpha_4^* + \beta_5\alpha_5^*\Big)*\\
	~ &= \Big(\alpha_1^*\beta_1 + \alpha_2^*\beta_2 + \alpha_3^*\beta_3 +
	\alpha_4^*\beta_4 + \alpha_5^*\beta_5\Big)*\\
	~ &= \Big(
		\begin{pmatrix}
			\alpha_1^* & \alpha_2^* & \alpha_3^* & \alpha_4^* & \alpha_5^* \\
		\end{pmatrix}
		\begin{pmatrix}
			\beta_1 \\
			\beta_2 \\
			\beta_3 \\
			\beta_4 \\
			\beta_5 \\
		\end{pmatrix} \Big)^*\\
	~ &= \braket{A}{B}^* \qed
\end{align*}

\end{document}
