\documentclass[solutions.tex]{subfiles}

\xtitle

\begin{document}
\maketitle
\begin{exercise} Prove that if $M$ and $L$ are both
Hermitian, $i[M,L]$ is also Hermitian. Note that the $i$
is important. The commutator is, by itself, not Hermitian.
\end{exercise}
\begin{align*}
	(i[M, L])^\dagger &= \left(i(ML - LM\right))^\dagger && ~\\
	~ &= (iML-iLM)^\dagger && ~\\
	~ &= \left((iML-iLM)^T\right)^* && \text{($\dagger$'s definition)}\\
	~ &= \left((iML)^T-(iLM)^T\right)^* && \left((A+B)^T = A^T + B^T\right)\\
	~ &= \left(iL^TM^T-iM^TL^T\right)^* && \left((AB)^T = B^TA^T\right)\\
	~ &= \left(-i(L^TM^T)^*+i(M^TL^T)^*\right) &&
		\left((zt)^* = z^*t^*; (z+t)* = z^*+t^*)\right)\\
	~ &= i\left(M^\dagger L^\dagger-L^\dagger M^\dagger\right) &&
		\text{($\dagger$'s definition)}\\
	~ &= i\left(ML-LM\right) &&
		\left(L=L^\dagger; M=M^\dagger\right) \\
	~ &= i[M, L] && \qed \\
\end{align*}
\end{document}
