\documentclass[solutions.tex]{subfiles}

\xtitle{L03E03}

\begin{document}
\maketitle
\begin{exercise}
Show by differentiation that this satisfies the equation of motion.
\end{exercise}
Contrary to the previous exercice, instead of integrating to find
the solution, we start from the solution and climb back to our original
equation of motion, which are, in the case of a constant force $F_z$
applied to a mass $m$ following the $z$-axis:
\[
	v_z(t) = \dot{z}(t) = v_z(0) - \frac{F_z}{m}t
\]
The proposed solution is:
\[
	z(t) = z_0 + v_z(0)t + \frac{F_z}{2m}t^2
\]
Immediately, by derivation, constants goes to $0$, $t$ becomes $1$ and
$t^2$ becomes $2t$, we indeed obtain:
\[
	\boxed{\frac{d}{dt}z(t) = \dot{z}(t) = v_z(t) = v_z(0) + \frac{F_z}{m}t}\qed
\]
\end{document}
