\documentclass[solutions.tex]{subfiles}

\xtitle

\begin{document}
\maketitle
\begin{exercise}
Show that the vector potentials in Equations $(8)$ and
Equations $(9)$ both give the same uniform magnetic field. This
means that the two differ by a gradient. Find the scalar whose
gradient, when added to Equations $(8)$, gives Equations $(9)$.
\end{exercise}

We're in the context of exploring how a magnetic field $\bm{B}$
\textit{must} "derive" from vector potential $\bm{A}$:
\[
	\bm{B} = \bm\nabla\times\bm{A}
\]

That is:
\[
	\bm{B} = \bm\nabla\times \bm{A} = \begin{pmatrix}
		\dfrac{\partial A_z}{\partial y} - \dfrac{\partial A_y}{\partial z} \\[1em]
		\dfrac{\partial A_x}{\partial z} - \dfrac{\partial A_z}{\partial x} \\[1em]
		\dfrac{\partial A_y}{\partial x} - \dfrac{\partial A_x}{\partial y}
	\end{pmatrix}
\]

Now the authors gave us two vector potential $\bm{A}$, $\bm{A}'$ in the
referenced Equations $(8)$ and $(9)$:
\[
	\bm{A} = \begin{pmatrix}
		0 \\
		b x \\
		0
	\end{pmatrix};\qquad \bm{A}' = \begin{pmatrix}
		-b y \\
		0 \\
		0
	\end{pmatrix}
\]

And we must prove that they correspond to an uniform magnetic field
pointing in the $z$ axis with intensity $b$ (i.e $\bm{B} = (0, 0, b)$)

We just have to compute the curl of $\bm{A}$ and $\bm{A}'$:
\[
	\bm\nabla\times \bm{A} = \begin{pmatrix}
		\dfrac{\partial A_z}{\partial y} - \dfrac{\partial A_y}{\partial z} \\[1em]
		\dfrac{\partial A_x}{\partial z} - \dfrac{\partial A_z}{\partial x} \\[1em]
		\dfrac{\partial A_y}{\partial x} - \dfrac{\partial A_x}{\partial y}
	\end{pmatrix} = \begin{pmatrix}
		0 - 0 \\
		0 - 0 \\
		b - 0
	\end{pmatrix} = \bm{B}\qed
\]
\[
	\bm\nabla\times \bm{A}' = \begin{pmatrix}
		\dfrac{\partial A'_z}{\partial y} - \dfrac{\partial A'_y}{\partial z} \\[1em]
		\dfrac{\partial A'_x}{\partial z} - \dfrac{\partial A'_z}{\partial x} \\[1em]
		\dfrac{\partial A'_y}{\partial x} - \dfrac{\partial A'_x}{\partial y}
	\end{pmatrix} = \begin{pmatrix}
		0 - 0 \\
		0 - 0 \\
		0 - (-b)
	\end{pmatrix} = \bm{B}\qed
\]

Now the two vector fields must differ by gradient field generate from some scalar
field $s(x, y, z)$:
\[
	\bm{A}' = \bm{A} + \bm\nabla s
\]
Which means
\[
	\bm\nabla s = \bm{A}'-\bm{A} = \begin{pmatrix}
		-by \\
		-bx \\
		0
	\end{pmatrix} = -b \begin{pmatrix}
		y \\
		x \\
		0
	\end{pmatrix} = \begin{pmatrix}
		\dfrac{\partial s}{\partial x} \\[1em]
		\dfrac{\partial s}{\partial y} \\[1em]
		\dfrac{\partial s}{\partial z}
	\end{pmatrix}
\]

We can "see" that $s(x, y, z) = -b xy$ fits:
\[
	\dfrac{\partial s}{\partial x} = -by;\qquad
	\dfrac{\partial s}{\partial y} = -bx
\]

\end{document}
